@prefix : <http://www.semanticweb.org/robertocannarella/ontologies/2021/1/ontologynarratives#> .
@prefix owl: <http://www.w3.org/2002/07/owl#> .
@prefix rdf: <http://www.w3.org/1999/02/22-rdf-syntax-ns#> .
@prefix xml: <http://www.w3.org/XML/1998/namespace> .
@prefix xsd: <http://www.w3.org/2001/XMLSchema#> .
@prefix rdfs: <http://www.w3.org/2000/01/rdf-schema#> .
@base <http://www.semanticweb.org/robertocannarella/ontologies/2021/1/ontologynarratives> .

<http://www.semanticweb.org/robertocannarella/ontologies/2021/1/ontologynarratives> rdf:type owl:Ontology .

#################################################################
#    Object Properties
#################################################################

###  http://www.semanticweb.org/robertocannarella/ontologies/2021/1/ontologynarratives#composes
:composes rdf:type owl:ObjectProperty ;
          owl:inverseOf :isComposedOf ;
          rdfs:domain :Event ;
          rdfs:range :Narrative ;
          rdfs:comment "It links an event to the narrative of which the event is part. An event may be the same in different narratives (e.g., an historical fact reported in more books), so the property has not been defined as functional."@en ;
          rdfs:label "composes"@en .


###  http://www.semanticweb.org/robertocannarella/ontologies/2021/1/ontologynarratives#creates
:creates rdf:type owl:ObjectProperty ;
         owl:inverseOf :isCreatedBy ;
         rdfs:domain :Narrator ;
         rdfs:range :Narrative ;
         rdfs:comment "It links a narrator to the narrative s/he has created. A narrator can create different narratives, so the property is not functional."@en ;
         rdfs:label "creates"@en .


###  http://www.semanticweb.org/robertocannarella/ontologies/2021/1/ontologynarratives#hasCharacter
:hasCharacter rdf:type owl:ObjectProperty ;
              rdfs:subPropertyOf :hasParticipant ;
              owl:inverseOf :isCharacterOf ;
              rdfs:domain :Event ;
              rdfs:range :Character ;
              owl:propertyDisjointWith :hasObject ;
              rdfs:comment "It links an event to its character(s). An event can have more than one participating character, thus, the property has not been defined as functional."@en ;
              rdfs:label "hasCharacter"@en .


###  http://www.semanticweb.org/robertocannarella/ontologies/2021/1/ontologynarratives#hasContractWith
:hasContractWith rdf:type owl:ObjectProperty ;
                 owl:inverseOf :offersContractTo ;
                 rdfs:domain :Narrator ;
                 rdfs:range :Publisher ;
                 owl:propertyChainAxiom ( :creates
                                          :isReportedIn
                                          :hasPublisher
                                        ) ;
                 rdfs:comment "It links a narrator to the publisher with which s/he has a contract."@en ;
                 rdfs:label "hasContractWith"@en .


###  http://www.semanticweb.org/robertocannarella/ontologies/2021/1/ontologynarratives#hasObject
:hasObject rdf:type owl:ObjectProperty ;
           rdfs:subPropertyOf :hasParticipant ;
           owl:inverseOf :isObjectOf ;
           rdfs:domain :Event ;
           rdfs:range :Object ;
           rdfs:comment "It links an event to its object(s). An event can have more than one participating object, thus, the property has not been defined as functional."@en ;
           rdfs:label "hasObject"@en .


###  http://www.semanticweb.org/robertocannarella/ontologies/2021/1/ontologynarratives#hasParticipant
:hasParticipant rdf:type owl:ObjectProperty ;
                rdfs:comment "hasParticipant is a superproperty of: hasCharacter, hasObject."@en ;
                rdfs:label "hasParticipant"@en .


###  http://www.semanticweb.org/robertocannarella/ontologies/2021/1/ontologynarratives#hasPublisher
:hasPublisher rdf:type owl:ObjectProperty ;
              owl:inverseOf :publishes ;
              rdf:type owl:FunctionalProperty ;
              rdfs:domain :Book ;
              rdfs:range :Publisher ;
              rdfs:comment "It links a book to the publisher that published it. A book can have only one publisher, so the property is functional."@en ;
              rdfs:label "hasPublisher"@en .


###  http://www.semanticweb.org/robertocannarella/ontologies/2021/1/ontologynarratives#hosts
:hosts rdf:type owl:ObjectProperty ;
       owl:inverseOf :occursIn ;
       rdf:type owl:InverseFunctionalProperty ;
       rdfs:domain :Location ;
       rdfs:range :Event ;
       rdfs:comment "It links a location to the event(s) which can take place in there. A location can be the setting of several events, so the property is not functional."@en ;
       rdfs:label "hosts"@en .


###  http://www.semanticweb.org/robertocannarella/ontologies/2021/1/ontologynarratives#isCharacterOf
:isCharacterOf rdf:type owl:ObjectProperty ;
               rdfs:subPropertyOf :isParticipantOf ;
               rdfs:domain :Character ;
               rdfs:range :Event ;
               owl:propertyDisjointWith :isObjectOf ;
               rdfs:comment "It links a character to the event in which s/he has taken part. One same character can take part in multiple events of a narrative, thus the property has not been defined as functional."@en ;
               rdfs:label "isCharacterOf"@en .


###  http://www.semanticweb.org/robertocannarella/ontologies/2021/1/ontologynarratives#isComposedOf
:isComposedOf rdf:type owl:ObjectProperty ;
              rdfs:domain :Narrative ;
              rdfs:range :Event ;
              rdfs:comment "It connects a narrative and the event(s) composing it. A narrative can be composed of more than one event, so the property is not functional."@en ;
              rdfs:label "isComposedOf"@en .


###  http://www.semanticweb.org/robertocannarella/ontologies/2021/1/ontologynarratives#isCreatedBy
:isCreatedBy rdf:type owl:ObjectProperty ;
             rdfs:domain :Narrative ;
             rdfs:range :Narrator ;
             rdfs:comment "It links a narrative to the narrator that has created it. One narrative can be created by multiple narrators, so the property is not functional."@en ;
             rdfs:label "isCreatedBy"@en .


###  http://www.semanticweb.org/robertocannarella/ontologies/2021/1/ontologynarratives#isObjectOf
:isObjectOf rdf:type owl:ObjectProperty ;
            rdfs:subPropertyOf :isParticipantOf ;
            rdfs:domain :Object ;
            rdfs:range :Event ;
            rdfs:comment "It links an object to the event in which it is present. One same object can take part in multiple events of a narrative, thus the property has not been defined as functional."@en ;
            rdfs:label "isObjectOf"@en .


###  http://www.semanticweb.org/robertocannarella/ontologies/2021/1/ontologynarratives#isParticipantOf
:isParticipantOf rdf:type owl:ObjectProperty ;
                 rdfs:comment "isParticipantOf is a superproperty of: isObjectOf, isCharacterOf."@en ;
                 rdfs:label "isParticipantOf"@en .


###  http://www.semanticweb.org/robertocannarella/ontologies/2021/1/ontologynarratives#isReportedIn
:isReportedIn rdf:type owl:ObjectProperty ;
              owl:inverseOf :reports ;
              rdfs:domain :Narrative ;
              rdfs:range :Book ;
              rdfs:comment "It links a narrative to the book in which it is reported. A narrative may be the same in more than one book, so the property is not functional."@en ;
              rdfs:label "isReportedIn"@en .


###  http://www.semanticweb.org/robertocannarella/ontologies/2021/1/ontologynarratives#occursIn
:occursIn rdf:type owl:ObjectProperty ,
                   owl:FunctionalProperty ;
          rdfs:domain :Event ;
          rdfs:range :Location ;
          rdfs:comment "It links an event to the location in which it occurs. The property is functional because an event can take place in exactly one place."@en ;
          rdfs:label "occursIn"@en .


###  http://www.semanticweb.org/robertocannarella/ontologies/2021/1/ontologynarratives#offersContractTo
:offersContractTo rdf:type owl:ObjectProperty ;
                  rdfs:domain :Publisher ;
                  rdfs:range :Narrator ;
                  rdfs:comment "It links a publisher to the narrator with whom it [the publisher] has established a contract."@en ;
                  rdfs:label "offersContractTo"@en .


###  http://www.semanticweb.org/robertocannarella/ontologies/2021/1/ontologynarratives#publishes
:publishes rdf:type owl:ObjectProperty ,
                    owl:InverseFunctionalProperty ;
           rdfs:domain :Publisher ;
           rdfs:range :Book ;
           rdfs:comment "It links a publisher to the books it publishes. A publisher publishes more than one book, so the property is not functional."@en ;
           rdfs:label "publishes"@en .


###  http://www.semanticweb.org/robertocannarella/ontologies/2021/1/ontologynarratives#reports
:reports rdf:type owl:ObjectProperty ;
         rdfs:domain :Book ;
         rdfs:range :Narrative ;
         rdfs:comment "It connects a book and the narrative(s) reported in it. The property is not functional because a book can report more than one narrative."@en ;
         rdfs:label "reports"@en .


###  http://www.semanticweb.org/robertocannarella/ontologies/2021/1/ontologynarratives#sellsBooksPublishedBy
:sellsBooksPublishedBy rdf:type owl:ObjectProperty ;
                       owl:inverseOf :sellsBooksThrough ;
                       rdfs:domain :Bookshop ;
                       rdfs:range :Publisher ;
                       rdfs:comment "It links a bookshop to the publisher of which it publishes books. A bookshop sells books by more than one publisher, so the property is not functional."@en ;
                       rdfs:label "sellsBooksBy"@en .


###  http://www.semanticweb.org/robertocannarella/ontologies/2021/1/ontologynarratives#sellsBooksThrough
:sellsBooksThrough rdf:type owl:ObjectProperty ;
                   rdfs:domain :Publisher ;
                   rdfs:range :Bookshop ;
                   rdfs:comment "It links a publisher to the bookshops through which its books are sold. These bookshops are more than one, so the property is not functional."@en ;
                   rdfs:label "sellsBooksThrough"@en .


#################################################################
#    Data properties
#################################################################

###  http://www.semanticweb.org/robertocannarella/ontologies/2021/1/ontologynarratives#hasBeginningDate
:hasBeginningDate rdf:type owl:DatatypeProperty ,
                           owl:FunctionalProperty ;
                  rdfs:domain :Event ;
                  rdfs:range xsd:dateTime ;
                  rdfs:comment "hasBeginningDate links an event to the date in which it begins, expressed using xsd:dateTime. The property is functional because an event can only start on one specific day."@en ;
                  rdfs:label "hasBeginningDate"@en .


###  http://www.semanticweb.org/robertocannarella/ontologies/2021/1/ontologynarratives#hasEndingDate
:hasEndingDate rdf:type owl:DatatypeProperty ,
                        owl:FunctionalProperty ;
               rdfs:domain :Event ;
               rdfs:range xsd:dateTime ;
               rdfs:comment "hasEndingDate links an event to the date in which it ends, expressed using xsd:dateTime. The property is functional because an event can only end on one specific day."@en ;
               rdfs:label "hasEndingDate"@en .


###  http://www.semanticweb.org/robertocannarella/ontologies/2021/1/ontologynarratives#hasID
:hasID rdf:type owl:DatatypeProperty ,
                owl:FunctionalProperty ;
       rdfs:domain :Publisher ;
       rdfs:range xsd:positiveInteger ;
       rdfs:comment "hasID links a publisher to its Identification Code (ID), expressed as a positive integer. It is functional because a publisher can have only one ID, which identifies it unambiguously."@en ;
       rdfs:label "hasID"@en .


###  http://www.semanticweb.org/robertocannarella/ontologies/2021/1/ontologynarratives#hasISBNCode
:hasISBNCode rdf:type owl:DatatypeProperty ,
                      owl:FunctionalProperty ;
             rdfs:domain :Book ;
             rdfs:range xsd:string ;
             rdfs:comment "hasISBNCode links a book to the ISBN code associated with it, expressed as a string. It is functional because an ISBN code is distinctive of one particular book, so a book cannot have more than one."@en ;
             rdfs:label "hasISBNCode"@en .


###  http://www.semanticweb.org/robertocannarella/ontologies/2021/1/ontologynarratives#hasName
:hasName rdf:type owl:DatatypeProperty ;
         rdfs:range xsd:string ;
         rdfs:comment "hasName is a superproperty of: hasCharacterName, hasLocationName, hasObjectName and hasPublisherName. These properties have been identified in order to provide a specific (and when needed, inferable) domain for each of them."@en ;
         rdfs:label "hasName"@en .


###  http://www.semanticweb.org/robertocannarella/ontologies/2021/1/ontologynarratives#hasNameCharacter
:hasNameCharacter rdf:type owl:DatatypeProperty ;
                  rdfs:subPropertyOf :hasName ;
                  rdfs:domain :Character ;
                  rdfs:range xsd:string ;
                  rdfs:label "hasNameCharacter"@en ,
                             "hasNameCharacter links a character to its name, expressed as a string. A character may have several names, which is why the property is not functional."@en .


###  http://www.semanticweb.org/robertocannarella/ontologies/2021/1/ontologynarratives#hasNameLocation
:hasNameLocation rdf:type owl:DatatypeProperty ;
                 rdfs:subPropertyOf :hasName ;
                 rdfs:domain :Location ;
                 rdfs:range xsd:string ;
                 rdfs:comment "hasNameLocation links a location to its name, expressed as a string. A location may have several names, which is why the property is not functional."@en ;
                 rdfs:label "hasNameLocation"@en .


###  http://www.semanticweb.org/robertocannarella/ontologies/2021/1/ontologynarratives#hasNameObject
:hasNameObject rdf:type owl:DatatypeProperty ;
               rdfs:subPropertyOf :hasName ;
               rdfs:domain :Object ;
               rdfs:range xsd:string ;
               rdfs:comment "hasNameObject links an object to its name, expressed as a string. An object may have several names, which is why the property is not functional."@en .


###  http://www.semanticweb.org/robertocannarella/ontologies/2021/1/ontologynarratives#hasPrice
:hasPrice rdf:type owl:DatatypeProperty ,
                   owl:FunctionalProperty ;
          rdfs:domain :Book ;
          rdfs:range xsd:positiveInteger ;
          rdfs:comment "hasPrice links a book to its price, expressed as a positive integer. It is functional because a book can have only one price."@en ;
          rdfs:label "hasPrice"@en .


###  http://www.semanticweb.org/robertocannarella/ontologies/2021/1/ontologynarratives#hasPublisherName
:hasPublisherName rdf:type owl:DatatypeProperty ;
                  rdfs:subPropertyOf :hasName ;
                  rdf:type owl:FunctionalProperty ;
                  rdfs:domain :Publisher ;
                  rdfs:range xsd:string ;
                  rdfs:comment "hasNamePublisher links a publisher to its name, expressed as a string. The name of a publisher identifies it, so the property is functional (it can only be one)."@en ;
                  rdfs:label "hasNamePublisher"@en .


###  http://www.semanticweb.org/robertocannarella/ontologies/2021/1/ontologynarratives#hasTitle
:hasTitle rdf:type owl:DatatypeProperty ;
          rdfs:domain :Book ;
          rdfs:range xsd:string ;
          rdfs:comment "hasTitle links a book to the title (or titles) associated with it, expressed as a string."@en ;
          rdfs:label "hasTitle"@en .


#################################################################
#    Classes
#################################################################

###  http://www.semanticweb.org/robertocannarella/ontologies/2021/1/ontologynarratives#Book
:Book rdf:type owl:Class ;
      rdfs:subClassOf [ rdf:type owl:Restriction ;
                        owl:onProperty :reports ;
                        owl:someValuesFrom :Narrative
                      ] ,
                      [ rdf:type owl:Restriction ;
                        owl:onProperty :hasPublisher ;
                        owl:qualifiedCardinality "1"^^xsd:nonNegativeInteger ;
                        owl:onClass :Publisher
                      ] ,
                      [ rdf:type owl:Restriction ;
                        owl:onProperty :hasTitle ;
                        owl:someValuesFrom xsd:string
                      ] ,
                      [ rdf:type owl:Restriction ;
                        owl:onProperty :hasISBNCode ;
                        owl:qualifiedCardinality "1"^^xsd:nonNegativeInteger ;
                        owl:onDataRange xsd:string
                      ] ,
                      [ rdf:type owl:Restriction ;
                        owl:onProperty :hasPrice ;
                        owl:qualifiedCardinality "1"^^xsd:nonNegativeInteger ;
                        owl:onDataRange xsd:positiveInteger
                      ] ;
      rdfs:comment "A book is a resource that reports one or more narratives, that has a title, that is published by a publisher, that is identified by an ISBN code and that has a price."@en ;
      rdfs:label "Book"@en .


###  http://www.semanticweb.org/robertocannarella/ontologies/2021/1/ontologynarratives#Bookshop
:Bookshop rdf:type owl:Class ;
          rdfs:comment "A bookshop is a shop that sells books."@en ;
          rdfs:label "Bookshop"@en .


###  http://www.semanticweb.org/robertocannarella/ontologies/2021/1/ontologynarratives#Character
:Character rdf:type owl:Class ;
           rdfs:subClassOf :Participant ,
                           [ rdf:type owl:Restriction ;
                             owl:onProperty :hasNameCharacter ;
                             owl:someValuesFrom xsd:string
                           ] ;
           owl:disjointWith :Object ;
           owl:disjointUnionOf ( :HumanCharacter
                                 :NotHumanCharacter
                               ) ;
           rdfs:comment "A character is a kind of participant. A character has a name and can be either a human character or a not human character."@en ;
           rdfs:label "Character"@en .


###  http://www.semanticweb.org/robertocannarella/ontologies/2021/1/ontologynarratives#Event
:Event rdf:type owl:Class ;
       rdfs:subClassOf [ rdf:type owl:Restriction ;
                         owl:onProperty :hasParticipant ;
                         owl:minQualifiedCardinality "1"^^xsd:nonNegativeInteger ;
                         owl:onClass :Participant
                       ] ,
                       [ rdf:type owl:Restriction ;
                         owl:onProperty :occursIn ;
                         owl:qualifiedCardinality "1"^^xsd:nonNegativeInteger ;
                         owl:onClass :Location
                       ] ,
                       [ rdf:type owl:Restriction ;
                         owl:onProperty :hasBeginningDate ;
                         owl:qualifiedCardinality "1"^^xsd:nonNegativeInteger ;
                         owl:onDataRange xsd:dateTime
                       ] ,
                       [ rdf:type owl:Restriction ;
                         owl:onProperty :hasEndingDate ;
                         owl:qualifiedCardinality "1"^^xsd:nonNegativeInteger ;
                         owl:onDataRange xsd:dateTime
                       ] ;
       rdfs:comment "An event is the fundamental portion of a narrative. It has one or more participants involved (be they characters or objects), it occurs in one location (be it real or fictional) and it has a starting date and an ending date."@en ;
       rdfs:label "Event"@en .


###  http://www.semanticweb.org/robertocannarella/ontologies/2021/1/ontologynarratives#FictionalLocation
:FictionalLocation rdf:type owl:Class ;
                   rdfs:subClassOf :Location ;
                   owl:disjointWith :RealLocation ;
                   rdfs:comment "A fictional location is a location of fantasy where events take place."@en ;
                   rdfs:label "Fictional Location"@en .


###  http://www.semanticweb.org/robertocannarella/ontologies/2021/1/ontologynarratives#HumanCharacter
:HumanCharacter rdf:type owl:Class ;
                rdfs:subClassOf :Character ;
                owl:disjointWith :NotHumanCharacter ;
                rdfs:comment "A human character is a kind of character that is a human."@en ;
                rdfs:label "Human Character"@en .


###  http://www.semanticweb.org/robertocannarella/ontologies/2021/1/ontologynarratives#Location
:Location rdf:type owl:Class ;
          rdfs:subClassOf [ rdf:type owl:Restriction ;
                            owl:onProperty :hasNameLocation ;
                            owl:someValuesFrom xsd:string
                          ] ;
          rdfs:comment "A location is where an event takes place. It can be either a real location or a fictional location, and it has a name."@en ;
          rdfs:label "Location"@en .


###  http://www.semanticweb.org/robertocannarella/ontologies/2021/1/ontologynarratives#Narrative
:Narrative rdf:type owl:Class ;
           rdfs:subClassOf [ rdf:type owl:Restriction ;
                             owl:onProperty :isComposedOf ;
                             owl:allValuesFrom :Event
                           ] ,
                           [ rdf:type owl:Restriction ;
                             owl:onProperty :isComposedOf ;
                             owl:minQualifiedCardinality "1"^^xsd:nonNegativeInteger ;
                             owl:onClass :Event
                           ] ,
                           [ rdf:type owl:Restriction ;
                             owl:onProperty :isCreatedBy ;
                             owl:minQualifiedCardinality "1"^^xsd:nonNegativeInteger ;
                             owl:onClass :Narrator
                           ] ;
           rdfs:comment "A narrative is composed of one or more events and is created by at least one narrator."@en ;
           rdfs:label "Narrative"@en .


###  http://www.semanticweb.org/robertocannarella/ontologies/2021/1/ontologynarratives#Narrator
:Narrator rdf:type owl:Class ;
          rdfs:subClassOf [ rdf:type owl:Restriction ;
                            owl:onProperty :hasContractWith ;
                            owl:minQualifiedCardinality "1"^^xsd:nonNegativeInteger ;
                            owl:onClass :Publisher
                          ] ;
          rdfs:comment "A narrator is the one creating a narrative, and that has at least one contract with a publisher."@en ;
          rdfs:label "Narrator"@en .


###  http://www.semanticweb.org/robertocannarella/ontologies/2021/1/ontologynarratives#NotHumanCharacter
:NotHumanCharacter rdf:type owl:Class ;
                   rdfs:subClassOf :Character ;
                   rdfs:comment "A human character is a kind of character that is a human."@en ;
                   rdfs:label "Not Human Character"@en .


###  http://www.semanticweb.org/robertocannarella/ontologies/2021/1/ontologynarratives#Object
:Object rdf:type owl:Class ;
        rdfs:subClassOf :Participant ,
                        [ rdf:type owl:Restriction ;
                          owl:onProperty :hasNameObject ;
                          owl:someValuesFrom xsd:string
                        ] ;
        rdfs:comment "A character is a kind of participant. It has a  name."@en ;
        rdfs:label "Object"@en .


###  http://www.semanticweb.org/robertocannarella/ontologies/2021/1/ontologynarratives#Organisation
:Organisation rdf:type owl:Class ;
              rdfs:comment "An organisation is a resource that generally represents a company, such as a publisher (of which it is the superclass)."@en ;
              rdfs:label "Organisation"@en .


###  http://www.semanticweb.org/robertocannarella/ontologies/2021/1/ontologynarratives#Participant
:Participant rdf:type owl:Class ;
             rdfs:comment "A participant generally identifies a resource taking part in the events of a narrative. A participant can be either a character or an object, which are both subclasses."@en ;
             rdfs:label "Participant"@en .


###  http://www.semanticweb.org/robertocannarella/ontologies/2021/1/ontologynarratives#Publisher
:Publisher rdf:type owl:Class ;
           rdfs:subClassOf :Organisation ,
                           [ rdf:type owl:Restriction ;
                             owl:onProperty :publishes ;
                             owl:minQualifiedCardinality "2"^^xsd:nonNegativeInteger ;
                             owl:onClass :Book
                           ] ,
                           [ rdf:type owl:Restriction ;
                             owl:onProperty :sellsBooksThrough ;
                             owl:minQualifiedCardinality "2"^^xsd:nonNegativeInteger ;
                             owl:onClass :Bookshop
                           ] ,
                           [ rdf:type owl:Restriction ;
                             owl:onProperty :hasID ;
                             owl:qualifiedCardinality "1"^^xsd:nonNegativeInteger ;
                             owl:onDataRange xsd:positiveInteger
                           ] ,
                           [ rdf:type owl:Restriction ;
                             owl:onProperty :hasPublisherName ;
                             owl:qualifiedCardinality "1"^^xsd:nonNegativeInteger ;
                             owl:onDataRange xsd:string
                           ] ;
           rdfs:comment "A publisher is an organisation that is concerned with publishing books. It is identified by a name and an ID. A publisher publishes more than one book (i.e., at least 2) and sells its books through more than one bookshop (i.e., through at least 2)."@en ;
           rdfs:label "Publisher"@en .


###  http://www.semanticweb.org/robertocannarella/ontologies/2021/1/ontologynarratives#RealLocation
:RealLocation rdf:type owl:Class ;
              rdfs:subClassOf :Location ;
              rdfs:comment "A real location is a location of the real world where events take place."@en ;
              rdfs:label "Real Location"@en .


#################################################################
#    Individuals
#################################################################

###  http://www.semanticweb.org/robertocannarella/ontologies/2021/1/ontologynarratives#book1
:book1 rdf:type owl:NamedIndividual ,
                :Book ;
       :hasPublisher :publisher1 ;
       :reports :narrative1 ;
       :hasISBNCode "880790098X"^^xsd:string ;
       :hasPrice "10"^^xsd:positiveInteger ;
       :hasTitle "Madame Bovary"^^xsd:string ;
       rdfs:comment "This individual describes the book \"Madame Bovary\"."@en .


###  http://www.semanticweb.org/robertocannarella/ontologies/2021/1/ontologynarratives#book2
:book2 rdf:type owl:NamedIndividual ,
                :Book ;
       :hasPublisher :publisher2 ;
       :reports :narrative2 ,
                :narrative5 ;
       :hasISBNCode "8806218182"^^xsd:string ;
       :hasPrice "12"^^xsd:positiveInteger ;
       :hasTitle "Il giovane Holden"^^xsd:string ;
       rdfs:comment "This individual describes the book \"Il giovane Holden\" (\"The Catcher in the Rye\")."@en .


###  http://www.semanticweb.org/robertocannarella/ontologies/2021/1/ontologynarratives#book3
:book3 rdf:type owl:NamedIndividual ,
                :Book ;
       :hasPublisher :publisher2 ;
       :reports :narrative3 ;
       :hasISBNCode "8806248189"^^xsd:string ;
       :hasPrice "13"^^xsd:positiveInteger ;
       :hasTitle "1984"^^xsd:string ;
       rdfs:comment "This individual describes the book \"1984\" (\"Nineteen Eighty-Four\")."@en .


###  http://www.semanticweb.org/robertocannarella/ontologies/2021/1/ontologynarratives#book4
:book4 rdf:type owl:NamedIndividual ,
                :Book ;
       :hasPublisher :publisher1 ;
       :reports :narrative4 ;
       :hasISBNCode "8807900386"^^xsd:string ;
       :hasPrice "8"^^xsd:positiveInteger ;
       :hasTitle "Frankenstein"^^xsd:string ;
       rdfs:comment "This individual describes the book \"Frankenstein\" (\"Frankenstein; or, The Modern Prometheus\")."@en .


###  http://www.semanticweb.org/robertocannarella/ontologies/2021/1/ontologynarratives#bookshop1
:bookshop1 rdf:type owl:NamedIndividual ,
                    :Bookshop ;
           :sellsBooksPublishedBy :publisher1 ,
                                  :publisher2 .


###  http://www.semanticweb.org/robertocannarella/ontologies/2021/1/ontologynarratives#bookshop2
:bookshop2 rdf:type owl:NamedIndividual ,
                    :Bookshop ;
           :sellsBooksPublishedBy :publisher2 .


###  http://www.semanticweb.org/robertocannarella/ontologies/2021/1/ontologynarratives#bookshop3
:bookshop3 rdf:type owl:NamedIndividual ,
                    :Bookshop .


###  http://www.semanticweb.org/robertocannarella/ontologies/2021/1/ontologynarratives#character1
:character1 rdf:type owl:NamedIndividual ,
                     :HumanCharacter ;
            :isCharacterOf :event1 ;
            :hasNameCharacter "Emma Bovary"^^xsd:string .


###  http://www.semanticweb.org/robertocannarella/ontologies/2021/1/ontologynarratives#character2
:character2 rdf:type owl:NamedIndividual ,
                     :HumanCharacter ;
            :hasNameCharacter "Holden Caulfield"^^xsd:string .


###  http://www.semanticweb.org/robertocannarella/ontologies/2021/1/ontologynarratives#character3
:character3 rdf:type owl:NamedIndividual ,
                     :HumanCharacter ;
            :isCharacterOf :event3 ,
                           :event4 ;
            :hasNameCharacter "Winston Smith"^^xsd:string .


###  http://www.semanticweb.org/robertocannarella/ontologies/2021/1/ontologynarratives#character4
:character4 rdf:type owl:NamedIndividual ,
                     :HumanCharacter ;
            :hasNameCharacter "Julia"^^xsd:string .


###  http://www.semanticweb.org/robertocannarella/ontologies/2021/1/ontologynarratives#character5
:character5 rdf:type owl:NamedIndividual ,
                     :HumanCharacter ;
            :isCharacterOf :event5 ;
            :hasNameCharacter "Victor Frankenstein"^^xsd:string .


###  http://www.semanticweb.org/robertocannarella/ontologies/2021/1/ontologynarratives#character6
:character6 rdf:type owl:NamedIndividual ,
                     :NotHumanCharacter ;
            :hasNameCharacter "The Creature"^^xsd:string .


###  http://www.semanticweb.org/robertocannarella/ontologies/2021/1/ontologynarratives#event1
:event1 rdf:type owl:NamedIndividual ,
                 :Event ;
        :composes :narrative1 ;
        :hasCharacter :character1 ;
        :occursIn :location1 ;
        :hasBeginningDate "1848-01-03T00:00:00"^^xsd:dateTime ;
        :hasEndingDate "1848-01-05T00:00:00"^^xsd:dateTime .


###  http://www.semanticweb.org/robertocannarella/ontologies/2021/1/ontologynarratives#event2
:event2 rdf:type owl:NamedIndividual ,
                 :Event ;
        :hasCharacter :character2 ;
        :occursIn :location2 ;
        :hasBeginningDate "1945-12-23T00:00:00"^^xsd:dateTime ;
        :hasEndingDate "1945-12-25T00:00:00"^^xsd:dateTime .


###  http://www.semanticweb.org/robertocannarella/ontologies/2021/1/ontologynarratives#event3
:event3 rdf:type owl:NamedIndividual ,
                 :Event ;
        :composes :narrative3 ;
        :hasCharacter :character3 ;
        :hasObject :object1 ;
        :occursIn :location3 ;
        :hasBeginningDate "1984-03-17T00:00:00"^^xsd:dateTime ;
        :hasEndingDate "1984-03-25T00:00:00"^^xsd:dateTime .


###  http://www.semanticweb.org/robertocannarella/ontologies/2021/1/ontologynarratives#event4
:event4 rdf:type owl:NamedIndividual ,
                 :Event ;
        :composes :narrative3 ;
        :hasCharacter :character3 ,
                      :character4 ;
        :occursIn :location3 ;
        :hasBeginningDate "1985-03-01T16:00:00"^^xsd:dateTime ;
        :hasEndingDate "1985-03-01T17:00:00"^^xsd:dateTime .


###  http://www.semanticweb.org/robertocannarella/ontologies/2021/1/ontologynarratives#event5
:event5 rdf:type owl:NamedIndividual ,
                 :Event ;
        :hasCharacter :character5 ,
                      :character6 ;
        :hasObject :object2 ;
        :occursIn :location4 ;
        :hasBeginningDate "1705-10-04T00:00:00"^^xsd:dateTime ;
        :hasEndingDate "1705-10-05T00:00:00"^^xsd:dateTime .


###  http://www.semanticweb.org/robertocannarella/ontologies/2021/1/ontologynarratives#event6
:event6 rdf:type owl:NamedIndividual ,
                 :Event ;
        :composes :narrative4 ;
        :hasCharacter :character6 ;
        :occursIn :location4 ;
        :hasBeginningDate "1705-04-01T00:00:00"^^xsd:dateTime ;
        :hasEndingDate "1705-04-10T00:00:00"^^xsd:dateTime .


###  http://www.semanticweb.org/robertocannarella/ontologies/2021/1/ontologynarratives#event7
:event7 rdf:type owl:NamedIndividual ,
                 :Event ;
        :composes :narrative5 .


###  http://www.semanticweb.org/robertocannarella/ontologies/2021/1/ontologynarratives#location1
:location1 rdf:type owl:NamedIndividual ,
                    :RealLocation ;
           :hasNameLocation "Yonville"^^xsd:string .


###  http://www.semanticweb.org/robertocannarella/ontologies/2021/1/ontologynarratives#location2
:location2 rdf:type owl:NamedIndividual ,
                    :RealLocation ;
           :hasNameLocation "Pennsylvania"^^xsd:string .


###  http://www.semanticweb.org/robertocannarella/ontologies/2021/1/ontologynarratives#location3
:location3 rdf:type owl:NamedIndividual ,
                    :FictionalLocation ;
           :hosts :event3 ,
                  :event4 ;
           :hasNameLocation "London (Oceania)"^^xsd:string ;
           rdfs:comment "This individual refers to the fictional version of London created by Orwell, placed in Oceania."@en .


###  http://www.semanticweb.org/robertocannarella/ontologies/2021/1/ontologynarratives#location4
:location4 rdf:type owl:NamedIndividual ,
                    :RealLocation ;
           :hosts :event5 ;
           :hasNameLocation "Geneva"^^xsd:string .


###  http://www.semanticweb.org/robertocannarella/ontologies/2021/1/ontologynarratives#narrative1
:narrative1 rdf:type owl:NamedIndividual ,
                     :Narrative ;
            :isComposedOf :event1 ,
                          :event4 ;
            :isCreatedBy :narrator1 ;
            :isReportedIn :book1 .


###  http://www.semanticweb.org/robertocannarella/ontologies/2021/1/ontologynarratives#narrative2
:narrative2 rdf:type owl:NamedIndividual ,
                     :Narrative ;
            :isComposedOf :event2 ;
            :isCreatedBy :narrator2 ;
            :isReportedIn :book2 .


###  http://www.semanticweb.org/robertocannarella/ontologies/2021/1/ontologynarratives#narrative3
:narrative3 rdf:type owl:NamedIndividual ,
                     :Narrative ;
            :isComposedOf :event3 ,
                          :event4 ;
            :isCreatedBy :narrator3 ;
            :isReportedIn :book3 .


###  http://www.semanticweb.org/robertocannarella/ontologies/2021/1/ontologynarratives#narrative4
:narrative4 rdf:type owl:NamedIndividual ,
                     :Narrative ;
            :isComposedOf :event5 ;
            :isCreatedBy :narrator4 ;
            :isReportedIn :book4 .


###  http://www.semanticweb.org/robertocannarella/ontologies/2021/1/ontologynarratives#narrative5
:narrative5 rdf:type owl:NamedIndividual ,
                     :Narrative ;
            :isCreatedBy :narrator2 ;
            :isReportedIn :book2 .


###  http://www.semanticweb.org/robertocannarella/ontologies/2021/1/ontologynarratives#narrator1
:narrator1 rdf:type owl:NamedIndividual ,
                    :Narrator ;
           :hasContractWith :publisher1 .


###  http://www.semanticweb.org/robertocannarella/ontologies/2021/1/ontologynarratives#narrator2
:narrator2 rdf:type owl:NamedIndividual ,
                    :Narrator ;
           :creates :narrative2 ,
                    :narrative5 ;
           :hasContractWith :publisher2 .


###  http://www.semanticweb.org/robertocannarella/ontologies/2021/1/ontologynarratives#narrator3
:narrator3 rdf:type owl:NamedIndividual ,
                    :Narrator ;
           :hasContractWith :publisher2 .


###  http://www.semanticweb.org/robertocannarella/ontologies/2021/1/ontologynarratives#narrator4
:narrator4 rdf:type owl:NamedIndividual ,
                    :Narrator .


###  http://www.semanticweb.org/robertocannarella/ontologies/2021/1/ontologynarratives#object1
:object1 rdf:type owl:NamedIndividual ,
                  :Object ;
         :isObjectOf :event3 ;
         :hasNameObject "Propaganda Poster"^^xsd:string .


###  http://www.semanticweb.org/robertocannarella/ontologies/2021/1/ontologynarratives#object2
:object2 rdf:type owl:NamedIndividual ,
                  :Object ;
         :hasNameObject "Victor's journal"^^xsd:string .


###  http://www.semanticweb.org/robertocannarella/ontologies/2021/1/ontologynarratives#publisher1
:publisher1 rdf:type owl:NamedIndividual ,
                     :Publisher ;
            :offersContractTo :narrator1 ;
            :publishes :book1 ,
                       :book4 ;
            :sellsBooksThrough :bookshop1 ,
                               :bookshop2 ;
            :hasID "4998"^^xsd:positiveInteger ;
            :hasPublisherName "Feltrinelli"^^xsd:string .


###  http://www.semanticweb.org/robertocannarella/ontologies/2021/1/ontologynarratives#publisher2
:publisher2 rdf:type owl:NamedIndividual ,
                     :Publisher ;
            :publishes :book2 ,
                       :book3 ;
            :sellsBooksThrough :bookshop2 ,
                               :bookshop3 ;
            :hasID "9962"^^xsd:positiveInteger ;
            :hasPublisherName "Einaudi"^^xsd:string .


#################################################################
#    General axioms
#################################################################

[ rdf:type owl:AllDisjointClasses ;
  owl:members ( :Book
                :Bookshop
                :Event
                :Location
                :Narrative
                :Narrator
                :Organisation
                :Participant
              )
] .


[ rdf:type owl:AllDifferent ;
  owl:distinctMembers ( :book1
                        :book2
                        :book3
                        :book4
                      )
] .


[ rdf:type owl:AllDifferent ;
  owl:distinctMembers ( :bookshop1
                        :bookshop2
                        :bookshop3
                      )
] .


[ rdf:type owl:AllDifferent ;
  owl:distinctMembers ( :character1
                        :character2
                        :character3
                        :character4
                        :character5
                        :character6
                      )
] .


[ rdf:type owl:AllDifferent ;
  owl:distinctMembers ( :event1
                        :event2
                        :event3
                        :event4
                        :event5
                        :event6
                        :event7
                      )
] .


[ rdf:type owl:AllDifferent ;
  owl:distinctMembers ( :location1
                        :location2
                        :location3
                        :location4
                      )
] .


[ rdf:type owl:AllDifferent ;
  owl:distinctMembers ( :narrative1
                        :narrative2
                        :narrative3
                        :narrative4
                        :narrative5
                      )
] .


[ rdf:type owl:AllDifferent ;
  owl:distinctMembers ( :narrator1
                        :narrator2
                        :narrator3
                        :narrator4
                      )
] .


[ rdf:type owl:AllDifferent ;
  owl:distinctMembers ( :object1
                        :object2
                      )
] .


[ rdf:type owl:AllDifferent ;
  owl:distinctMembers ( :publisher1
                        :publisher2
                      )
] .


###  Generated by the OWL API (version 4.5.9.2019-02-01T07:24:44Z) https://github.com/owlcs/owlapi
